Semantic/Capybara/Safety.lean
@@ -12,7 +12,7 @@ def Sig.platform_of : Nat -> Sig
 /-- A platform context with `n` ground capabilities. -/
 def Ctx.platform_of : (n : Nat) -> Ctx (Sig.platform_of n)
 | 0 => .empty
-| n+1 => ((Ctx.platform_of n),C<:.unbound),x:(.capt (.cvar .here) .cap)
+| n+1 => ((Ctx.platform_of n),C<:.unbound),x:(.capt (.cvar .epsilon .here) .cap)
 
 /-- A platform heap with `n` ground capabilities (basic capabilities). -/
 def Heap.platform_of (N : Nat) : Heap :=
@@ -42,11 +42,11 @@ def CaptureSet.to_platform_capability_set : CaptureSet (Sig.platform_of N) -> Ca
 | .empty => .empty
 | .union cs1 cs2 =>
     (cs1.to_platform_capability_set) ∪ (cs2.to_platform_capability_set)
-| .var x =>
+| .var _m x =>
     match x with
     | .bound b => .cap (b.level / 2)
     | .free n => .cap n
-| .cvar c => .cap (c.level / 2)
+| .cvar _m c => .cap (c.level / 2)
 
 /-- Type environment for a platform with `N` ground capabilities.
   Maps each pair `(C, x)` to capability `i` at heap location `i`:
@@ -54,7 +54,7 @@ def CaptureSet.to_platform_capability_set : CaptureSet (Sig.platform_of N) -> Ca
   term variable `x` maps to heap location `i`. -/
 def TypeEnv.platform_of : (N : Nat) -> TypeEnv (Sig.platform_of N)
 | 0 => .empty
-| N+1 => ((TypeEnv.platform_of N).extend_cvar (.var (.free N))).extend_var N
+| N+1 => ((TypeEnv.platform_of N).extend_cvar (.var .epsilon (.free N))).extend_var N
 
 /-- The platform heap is well-formed: it contains only capabilities, no values. -/
 theorem Heap.platform_of_wf (N : Nat) : (Heap.platform_of N).WfHeap := by
@@ -255,7 +255,7 @@ theorem TypeEnv.lookup_var_platform {x : BVar (Sig.platform_of N) .var} :
 
 /-- Lookup of capture variable in platform environment. -/
 theorem TypeEnv.lookup_cvar_platform {c : BVar (Sig.platform_of N) .cvar} :
-  (TypeEnv.platform_of N).lookup_cvar c = .var (.free (c.level / 2)) := by
+  (TypeEnv.platform_of N).lookup_cvar c = .var .epsilon (.free (c.level / 2)) := by
   induction N with
   | zero =>
     -- No capture variables in empty signature
@@ -363,7 +363,7 @@ theorem capture_set_denot_eq_platform {C : CaptureSet (Sig.platform_of N)}
       unfold CaptureSet.subst CaptureSet.to_platform_capability_set CaptureSet.ground_denot
       unfold CaptureSet.denot at ih1 ih2
       rw [ih1 hwf1, ih2 hwf2]
-  | var x =>
+  | var m x =>
     -- Variable (term variable used as capture)
     unfold CaptureSet.subst CaptureSet.to_platform_capability_set
     cases x with
@@ -394,7 +394,7 @@ theorem capture_set_denot_eq_platform {C : CaptureSet (Sig.platform_of N)}
           case isFalse => contradiction
         rw [reachability_of_loc_platform hn]
         rfl
-  | cvar c =>
+  | cvar m c =>
     -- Capture variable
     unfold CaptureSet.subst CaptureSet.to_platform_capability_set
     simp only [Subst.from_TypeEnv]
